and_and_or solver almost complete

src/Practice/practice3.lean
@@ -2,7 +2,47 @@
 The aim here is to write a solver that can handle ∨ and ∧ in both hypotheses and goals.
 This requires dealing with multiple goals. -/
 
-meta def tactic.interactive.main_tactic : tactic unit := sorry
+open tactic
+open list
+open expr
+
+meta def and_and_or : list expr → list expr → expr → tactic unit
+-- first argument is list of hypotheses yet to be processed
+-- second argument is target
+| (cons h t) (cons `(%%a ∨ %%b) u) e := sorry
+| (cons h t) (cons `(%%a ∧ %%b) u) e :=
+do nm₁ ← get_unused_name `h,
+  nm₂ ← get_unused_name `h,
+  ea ← to_expr ``(and.left %%h),
+  eb ← to_expr ``(and.right %%h),
+  ha ← assertv nm₁ a ea,
+  hb ← assertv nm₂ b eb,
+  clear h,
+  and_and_or
+    (cons ha (cons hb t))
+    (cons a (cons b u))
+    e
+| (cons _ t) (cons _ u) e := and_and_or t u e
+| nil (cons _ t) _ := fail "Unsynchronized lists as arguments to and_and_or"
+| (cons _ t) nil _ := fail "Unsynchronized lists as arguments to and_and_or"
+| nil nil `(%%a ∨ %%b) :=
+  (applyc ``or.inl >> and_and_or nil nil a) <|>
+  (applyc ``or.inr >> and_and_or nil nil b)
+| nil nil `(%%a ∧ %%b) :=
+  seq' (applyc ``and.intro) (target >>= and_and_or nil nil)
+| nil nil _ := assumption
+
+meta def tactic.interactive.main_tactic : tactic unit :=
+do t ← target,
+  l ← local_context,
+  tps ← l.mmap infer_type,
+  and_and_or l tps t
+
+example (P Q R : Prop) (h₁ : P) (h₂ : Q ∧ R): (P ∧ Q ∧ R) :=
+by main_tactic
+
+example (P Q R : Prop) (h : Q ∧ R) : (P ∨ Q ∨ R) :=
+by main_tactic
 
 example (P Q R : Prop) (h : (P ∨ Q) ∧ (P ∨ R)) : (P ∨ Q ∧ R) :=
-by sorry
+by main_tactic
